Fix transition relation using right_step, define left and right configs, prove some properties about the transition relation

Escallon/Two_way_DFA_HF.thy
@@ -72,7 +72,7 @@ abbreviation steps :: "'a config \<Rightarrow> 'a config \<Rightarrow> bool" (in
   "steps \<equiv> step\<^sup>*\<^sup>*"
 
 (*Induction rule analogous to rtranclp_induct2*)
-lemmas config_induct = 
+lemmas rtranclp_induct3 = 
   rtranclp_induct[of _ "(ax, ay, az)" "(bx, by, bz)", split_rule, consumes 1, case_names refl step]
 
 abbreviation reachable :: "'a list \<Rightarrow> 'a config \<Rightarrow> bool" (infix \<open>\<rightarrow>**\<close> 55) where
@@ -84,7 +84,7 @@ definition language :: "'a list set" where
 lemma unchanged_final:
   assumes "p = acc M \<or> p = rej M"
   shows "(u, p, v) \<rightarrow>* (u', q, v') \<Longrightarrow> p = q"
-proof (induction rule: config_induct)
+proof (induction rule: rtranclp_induct3)
   case (step a q' b c q'' d)
   then show ?case using assms
     by (smt (verit, ccfv_SIG) dfa2_axioms dfa2_def prod.inject step_foldedE)
@@ -92,7 +92,7 @@ qed simp
 
 lemma unchanged_substrings:
   "(u, q, v) \<rightarrow>* (u', p, v') \<Longrightarrow> rev u @ v = rev u' @ v'"
-proof (induction rule: config_induct) 
+proof (induction rule: rtranclp_induct3) 
   case (step a q' b c q'' d)
   then obtain p' d' where qd_def: "nxt M q' (hd b) = (p', d')" by fastforce
   consider "d' = Left" | "d' = Right"
@@ -120,12 +120,12 @@ lemma steps_app':
   shows "(ws, q, u) \<rightarrow>* (xs, q', []) \<Longrightarrow> (ws, q, u @ v) \<rightarrow>* (ys, p, zs)"
    (*both config rules break here and raw rtranclp_induct does not work either
       (Solved below)*)
-proof (induction arbitrary: ws q u rule: config_induct)
+proof (induction arbitrary: ws q u rule: rtranclp_induct3)
   oops
 
 lemma steps_app:
   "(u, q, v) \<rightarrow>* (u', p, v') \<Longrightarrow> (u, q, v @ xs) \<rightarrow>* (u', p, v' @ xs)"
-proof (induction rule: config_induct)
+proof (induction rule: rtranclp_induct3)
   case (step w q' x y p' z)
   from step(2) have "(w, q', x @ xs) \<rightarrow> (y, p', z @ xs)" by fastforce
   then show ?case using step(3) by simp
@@ -148,18 +148,23 @@ locale dfa2_transition = dfa2 + (*there's probably a better alternative than a s
   assumes "x \<noteq> []"
 begin 
 
+definition left_config :: "'a config \<Rightarrow> bool" where
+  "left_config c \<equiv> \<exists>u q v. c = (u, q, v) \<and> length u < length (\<langle>x\<langle>)"
+
+definition right_config :: "'a config \<Rightarrow> bool" where
+  "right_config c \<equiv> \<exists>u q v. c = (u, q, v) \<and> length u \<ge> length (\<langle>x\<langle>)"
+
 inductive left_step :: "'a config \<Rightarrow> 'a config \<Rightarrow> bool" (infix \<open>\<rightarrow>\<^sup>L\<close> 55) where
-  lstep [intro]: "\<lbrakk>x @ z \<rightarrow>** (ys, q, zs); (ys, q, zs) \<rightarrow> (ys', p, zs')
-                  ; length ys < length (\<langle>x\<langle>); length ys' < length (\<langle>x\<langle>)\<rbrakk> 
-      \<Longrightarrow> (ys, q, zs) \<rightarrow>\<^sup>L (ys', p, zs')"
+  lstep [intro]: "\<lbrakk>x @ z \<rightarrow>** c1; c1 \<rightarrow> c2; left_config c1; left_config c2\<rbrakk> 
+      \<Longrightarrow> c1 \<rightarrow>\<^sup>L c2"
 
 inductive_cases lstepE [elim]: "c1 \<rightarrow>\<^sup>L c2"
 
 (*A right_step definition seems to be necessary to define T*)
 inductive right_step :: "'a config \<Rightarrow> 'a config \<Rightarrow> bool" (infix \<open>\<rightarrow>\<^sup>R\<close> 55) where
-  rstep [intro]: "\<lbrakk>x @ z \<rightarrow>** (ys, q, zs); (ys, q, zs) \<rightarrow> (ys', p, zs')
-                  ; length ys \<ge> length (\<langle>x\<langle>); length ys' \<ge> length (\<langle>x\<langle>)\<rbrakk> 
-      \<Longrightarrow> (ys, q, zs) \<rightarrow>\<^sup>R (ys', p, zs')"
+  rstep [intro]: "\<lbrakk>x @ z \<rightarrow>** c1; c1 \<rightarrow> c2;
+                  right_config c1; right_config c2\<rbrakk> 
+      \<Longrightarrow> c1 \<rightarrow>\<^sup>R c2"
 
 inductive_cases rstepE [elim]: "c1 \<rightarrow>\<^sup>R c2"
 
@@ -175,8 +180,15 @@ abbreviation right_steps :: "'a config \<Rightarrow> 'a config \<Rightarrow> boo
   "right_steps \<equiv> right_step\<^sup>*\<^sup>*"
 
 abbreviation left_reachable :: "'a list \<Rightarrow> 'a config \<Rightarrow> bool" (infix \<open>\<rightarrow>\<^sup>L**\<close> 55) where
-  "w \<rightarrow>\<^sup>L** c \<equiv> ([], init M, \<langle>w\<rangle>) \<rightarrow>\<^sup>L* c" 
-(*Right reachability?*)
+  "w \<rightarrow>\<^sup>L** c \<equiv> \<exists>z. w = x @ z \<and>  ([], init M, \<langle>w\<rangle>) \<rightarrow>\<^sup>L* c" 
+(*TODO: Check*)
+
+inductive right_reachable :: "'a config \<Rightarrow> 'a config \<Rightarrow> bool" (infix \<open>\<rightarrow>\<^sup>R**\<close> 55) where
+  "\<lbrakk>\<langle>x\<rangle> = a # xs; x @ z \<rightarrow>** c1; 
+    c1 \<rightarrow>\<^sup>L* (rev xs, p, a # \<rangle>z\<rangle>); (rev xs, p, a # \<rangle>z\<rangle>) \<rightarrow> (rev (\<langle>x\<langle>), p', \<rangle>z\<rangle>);
+    (rev (\<langle>x\<langle>), p', \<rangle>z\<rangle>) \<rightarrow>\<^sup>R* c2\<rbrakk> \<Longrightarrow> c1 \<rightarrow>\<^sup>R** c2"
+ (*Right reachability: c1 is reachable and can reach c2 with a single boundary crossing
+    (is reachability of c1 too weak?)*)
 
 
 lemma left_steps_impl_steps [elim]:
@@ -184,7 +196,7 @@ lemma left_steps_impl_steps [elim]:
   obtains "c1 \<rightarrow>* c2" (*Is this bad usage of obtains? I
                        used it in order to be able to use this as an elim rule
                       if it is not: when in general to use elims?*)
-proof 
+proof
   from assms show "c1 \<rightarrow>* c2"
     by (induction rule: rtranclp_induct) auto
 qed
@@ -198,20 +210,23 @@ proof
 qed
 
 lemma left_steps_impl_lt_x: 
-  "\<lbrakk>(ys, q, zs) \<rightarrow>\<^sup>L* (ys', p, zs'); length ys < length (\<langle>x\<langle>)\<rbrakk> 
-    \<Longrightarrow> length ys' < length (\<langle>x\<langle>)"
-  by (induction rule: config_induct) auto
+  "\<lbrakk>c1 \<rightarrow>\<^sup>L* c2; left_config c1\<rbrakk> 
+    \<Longrightarrow> left_config c2"
+  by (induction rule: rtranclp_induct) auto
+  
 
 lemma right_steps_impl_ge_x: 
-  "\<lbrakk>(ys, q, zs) \<rightarrow>\<^sup>R* (ys', p, zs'); length ys \<ge> length (\<langle>x\<langle>)\<rbrakk> 
-    \<Longrightarrow> length ys' \<ge> length (\<langle>x\<langle>)"
-  by (induction rule: config_induct) auto
+  "\<lbrakk>c1 \<rightarrow>\<^sup>R* c2; right_config c1\<rbrakk> 
+    \<Longrightarrow> right_config c2"
+  by (induction rule: rtranclp_induct) auto
 
 proposition list_deconstruct1:
   assumes "m \<le> length xs"
   obtains ys zs where "length ys = m" "ys @ zs = xs" using assms 
   by (metis add_diff_cancel_right' append_take_drop_id le_iff_add length_drop 
       length_rev rev_eq_append_conv)
+(*This lemma was necessary for star_lstar_impl_substring_x but sledgehammer somehow was not able to 
+prove it locally. How to deal with this?*)
 
 proposition list_deconstruct2:
   assumes "m \<le> length xs"
@@ -226,10 +241,6 @@ qed
 
 lemmas list_deconstruct = list_deconstruct1 list_deconstruct2
 
-(*This lemma was necessary for the next one but sledgehammer somehow was not able to 
-prove it locally. How to deal with this?*)
-
-find_theorems "_ < _ \<Longrightarrow> _ \<le> _"
 
 lemma star_lstar_impl_substring_x:
   assumes nsteps: "x @ z \<rightarrow>** (xs, q, zs)"
@@ -237,15 +248,18 @@ lemma star_lstar_impl_substring_x:
       and lsteps: "(xs, q, zs) \<rightarrow>\<^sup>L* (as, p, bs)"
   obtains u where " rev as @ u = \<langle>x\<langle>" "u @ \<rangle>z\<rangle> = bs" 
 proof -
+  have leftconfig: "left_config (xs, q, zs)" unfolding left_config_def using in_x by blast
+  hence as_lt_x: "length as < length (\<langle>x\<langle>)" using lsteps
+    using left_config_def left_steps_impl_lt_x by force
   from lsteps show thesis
-  proof (induction arbitrary: xs q zs rule: config_induct)
+  proof (induction arbitrary: xs q zs rule: rtranclp_induct3)
     case refl 
     from unchanged_word nsteps lsteps have app: "\<langle>x @ z\<rangle> = rev as @ bs"
       by (metis left_steps_impl_steps unchanged_substrings)
-    moreover from this left_steps_impl_lt_x[OF lsteps in_x]
+    moreover from this as_lt_x
     obtain x' where "rev as @ x' = \<langle>x\<langle>" "x' @ \<rangle>z\<rangle> = bs"
     proof -
-      from left_steps_impl_lt_x[OF lsteps in_x] list_deconstruct1
+      from as_lt_x list_deconstruct1
       obtain xs xs' where "length xs = length as" and xapp: "xs @ xs' = \<langle>x\<langle>"
         using Nat.less_imp_le_nat by metis
       moreover from this have "length (xs' @ \<rangle>z\<rangle>) = length bs" using app 
@@ -275,19 +289,22 @@ lemma star_rstar_impl_substring_z:
       and rsteps: "(xs, q, zs) \<rightarrow>\<^sup>R* (as, p, bs)"
     obtains u where " rev (\<langle>x\<langle> @ u) = as" "u @ bs = \<rangle>z\<rangle>"
 proof -
+  have "right_config (xs, q, zs)" using not_in_x right_config_def by simp
+  with rsteps right_config_def have as_ge_x: "length (\<langle>x\<langle>) \<le> length as"
+    using right_steps_impl_ge_x by force
   from rsteps show thesis
-  proof (induction arbitrary: xs q zs rule: config_induct)
+  proof (induction arbitrary: xs q zs rule: rtranclp_induct3)
     case refl
     from unchanged_word nsteps rsteps have app: "\<langle>x @ z\<rangle> = rev as @ bs"
       by (metis right_steps_impl_steps unchanged_substrings)
-    moreover from this right_steps_impl_ge_x[OF rsteps not_in_x]
+    moreover from this as_ge_x
     obtain x' where "rev (\<langle>x\<langle> @ x') = as" "x' @ bs = \<rangle>z\<rangle>"
     proof -
       have "length bs \<le> length (\<rangle>z\<rangle>)" 
       proof (rule ccontr)
         assume "\<not>?thesis"
         hence "length bs > length (\<rangle>z\<rangle>)" by simp
-        with right_steps_impl_ge_x[OF rsteps not_in_x]
+        with as_ge_x
         have "length (rev as @ bs) > length (\<langle>x @ z\<rangle>)" by simp
         thus False using app by (metis nat_less_le)
       qed
@@ -310,13 +327,13 @@ proof -
 qed
 
 inductive T :: transition where
-  "\<lbrakk>\<langle>x\<rangle> = a # xs; x @ z \<rightarrow>\<^sup>L** (rev xs, q, a # \<rangle>z\<rangle>); (rev xs, q, a # \<rangle>z\<rangle>) \<rightarrow> (rev (\<langle>x\<langle>), p, \<rangle>z\<rangle>)\<rbrakk>
+  init_tr: "\<lbrakk>\<langle>x\<rangle> = a # xs; x @ z \<rightarrow>\<^sup>L** (rev xs, q, a # \<rangle>z\<rangle>); (rev xs, q, a # \<rangle>z\<rangle>) \<rightarrow> (rev (\<langle>x\<langle>), p, \<rangle>z\<rangle>)\<rbrakk>
     \<Longrightarrow> T None (Some q)" |
-  "\<lbrakk>\<langle>x\<rangle> = a # xs;
-    (rev (\<langle>x\<langle>), q', \<rangle>z\<rangle>) \<rightarrow> (rev xs, q, a # \<rangle>z\<rangle>); 
-    (rev xs, q, a # \<rangle>z\<rangle>) \<rightarrow>\<^sup>L* (rev xs, p, a # \<rangle>z\<rangle>); 
-    (rev xs, p, a # \<rangle>z\<rangle>) \<rightarrow> (rev (\<langle>x\<langle>), q'', \<rangle>z\<rangle>)\<rbrakk> \<Longrightarrow> T (Some q) (Some p)"
-(*TODO: Fix definitions using rstep as well*)
+  some_tr: "\<lbrakk>\<langle>x\<rangle> = a # xs; right_config c; x @ z \<rightarrow>** c; c \<rightarrow>\<^sup>R* (rev (\<langle>x\<langle>), q', \<rangle>z\<rangle>); 
+    (rev (\<langle>x\<langle>), q', \<rangle>z\<rangle>) \<rightarrow> (rev xs, q, a # \<rangle>z\<rangle>); (rev xs, q, a # \<rangle>z\<rangle>) \<rightarrow>\<^sup>L* (rev xs, p, a # \<rangle>z\<rangle>); 
+    (rev xs, p, a # \<rangle>z\<rangle>) \<rightarrow> (rev (\<langle>x\<langle>), q'', \<rangle>z\<rangle>)\<rbrakk> \<Longrightarrow> T (Some q) (Some p)" |
+  no_tr:  "\<lbrakk>\<langle>x\<rangle> = a # xs; right_config c; x @ z \<rightarrow>** c; \<nexists>q. c \<rightarrow>* (rev (\<langle>x\<langle>), q, \<rangle>z\<rangle>)\<rbrakk>
+    \<Longrightarrow> T None None" (*TODO: BOT*)
 
 (*TODO: Set up automation for T*)
 
@@ -325,16 +342,51 @@ end
 context dfa2
 begin
 abbreviation "T \<equiv> dfa2_transition.T M"
-notation T ("T\<^sub>_")
+
+definition Tset :: "'a list \<Rightarrow> (state \<times> state) set" where
+  "Tset x \<equiv> {(q, p). q \<in> states M \<and> p \<in> states M \<and> T x (Some q) (Some p)}"
+(*TODO*)
+
+lemma Tset_card_upperbound:
+  shows "card (Tset x) \<le> card (states M) ^ 2"
+proof -
+  have "Tset x \<subseteq> states M \<times> states M" unfolding Tset_def by blast
+  thus ?thesis using Groups_Big.card_cartesian_product 
+    by (metis card_mono finite_cartesian_product local.finite power2_eq_square)
+qed
+
+lemma Tset_finite:
+  "finite (Tset x)" 
+proof -
+  from finite have "finite (states M \<times> states M)" by simp
+  moreover have "Tset x \<subseteq> states M \<times> states M" unfolding Tset_def by blast
+  ultimately show ?thesis unfolding Tset_def 
+    using rev_finite_subset by auto
+qed
+
+lemma Tset_finite_index:
+  "finite (UNIV // Tset x)" (*Nontrivial(?) and not proved in the book*)
+  sorry
+
+
+
+theorem two_way_dfa_lang_regular: (*Should this be inside a locale/context?*)
+  "regular language"
+proof - (*Book proof is rather informal - formalization might be quite more complicated 
+        than expected*)
+  fix x y
+  have imp: "Tset x = Tset y \<Longrightarrow> (\<forall>z. x @ z \<in> language \<longleftrightarrow> y @ z \<in> language)"
+    unfolding Tset_def sorry
+  moreover have "(\<forall>z. x @ z \<in> language \<longleftrightarrow> y @ z \<in> language) 
+             \<longleftrightarrow> (x, y) \<in> eq_app_right language" unfolding eq_app_right_def by simp
+  ultimately have "finite (UNIV // eq_app_right language)" using Tset_finite_index sorry
+  then show ?thesis using L3_1 by auto
+qed
   
 end
 
-
 (*TODO: formalize iff chain (Kozen, p. 126) top-down*)
 
-theorem two_way_dfa_lang_regular:
-  assumes "dfa2 M"
-  shows "regular (dfa2.language M)"
-  \<proof>
+
 
 end
